new/golang/theory/chan.v
@@ -1,7 +1,9 @@
 From Perennial.Helpers Require Import List.
 From New.golang.defn Require Export chan.
 From New.proof.github_com.goose_lang.goose.model.channel
-  Require Import chan_init chan_au_base chan_au_send chan_au_recv.
+  Require Export chan_au_base.
+From New.proof.github_com.goose_lang.goose.model.channel
+  Require Import chan_init chan_au_send chan_au_recv.
 From iris.base_logic Require Export lib.ghost_var.
 From New.golang.theory Require Export pre.
 From Perennial Require Import base.
